

# Proof of some fundamental relationships in survival analysis

Philip Fowler

June 10, 2025

## 1 Definitions

Let  $X$  be a continuous random variable measuring the time to some prespecified event. Then define the density function  $f(x)$ , the cumulative distribution function  $F(x)$ , the survival function  $S(x)$ , the hazard function  $h(x)$  and the cumulative hazard function as the following:

$$f(x) = \lim_{\Delta x \rightarrow 0} \frac{Pr(x \leq X < x + \Delta x)}{\Delta x}$$

$$F(x) = Pr(X \leq x) = \int_{-\infty}^x f(t)dt$$

$$S(x) = 1 - F(x) = Pr(X > x) = \int_x^{\infty} f(t)dt$$

$$h(x) = \lim_{\Delta x \rightarrow 0} \frac{Pr(x \leq X < x + \Delta x | X \geq x)}{\Delta x}$$

$$H(x) = \int_0^x h(t)dt$$

## 2 Relationships between the entities

We will now prove some well-know relationships between  $f(x)$ ,  $F(x)$ ,  $S(x)$ ,  $h(x)$  and  $H(x)$ .

**2.1**  $f(x) = -\frac{dS(x)}{dx}$

This follows directly from noting that  $S(x) = 1 - F(x)$  and that  $f(x) = dF(x)/dx$ . That is, by definition

$$f(x) = \frac{dF(x)}{dx} = \frac{d[1 - S(x)]}{dx} = -\frac{dS(x)}{dx}$$

Q.E.D.

**2.2**  $h(x) = f(x)/S(x)$

Remembering that  $Pr(A, B) = Pr(A|B)Pr(B)$  and that thus  $Pr(A|B) = Pr(A, B)/Pr(B)$  it follows that:

$$\lim_{\Delta x \rightarrow 0} \frac{Pr(x \leq X < x + \Delta x | X \geq x)}{\Delta x} = \lim_{\Delta x \rightarrow 0} \frac{Pr(x \leq X < x + \Delta x, X \geq x)}{\Delta x Pr(X \geq x)}$$

Noting that  $x \leq X$  is the same statement as  $X \geq x$ , it follows that

$$\lim_{\Delta x \rightarrow 0} \frac{Pr(x \leq X < x + \Delta x, X \geq x)}{\Delta x Pr(X \geq x)} = \lim_{\Delta x \rightarrow 0} \frac{Pr(x \leq X < x + \Delta x)}{\Delta x Pr(X \geq x)}$$

We now rewrite the right hand side for clarity:

$$\lim_{\Delta x \rightarrow 0} \frac{Pr(x \leq X < x + \Delta x)}{\Delta x Pr(X \geq x)} = \lim_{\Delta x \rightarrow 0} \frac{Pr(x \leq X < x + \Delta x)}{\Delta x} \frac{1}{Pr(X \geq x)}$$

From here we just use the definition of  $f(x)$  and  $S(x)$  and see that

$$\lim_{\Delta x \rightarrow 0} \frac{Pr(x \leq X < x + \Delta x)}{\Delta x} \frac{1}{Pr(X \geq x)} = f(x) \frac{1}{S(x)} = \frac{f(x)}{S(x)}$$

Q.E.D.

**2.3**  $h(x) = -\frac{d \ln[S(x)]}{dx}$

Remembering that  $S(x) = 1 - F(x)$  it follows that

$$-\frac{d \ln[S(x)]}{dx} = -\frac{d \ln[1 - F(x)]}{dx}$$

Next we recall the chain rule of differentiation, which states that for two functions  $f$  and  $g$ , it follows that  $\frac{df(g(x))}{dx} = \frac{df(g(x))}{dg(x)} \cdot \frac{dg(x)}{dx}$ . We also recall that the derivative of  $\ln x$  is  $1/x$ . Thus

$$-\frac{d \ln [1 - F(x)]}{dx} = -\frac{1}{1 - F(x)} \frac{d [1 - F(x)]}{dx}$$

The derivative of a sum is the sum of the derivatives. Thus

$$-\frac{1}{1 - F(x)} \frac{d [1 - F(x)]}{dx} = -\frac{1}{1 - F(x)} \left[ \frac{d1}{dx} - \frac{dF(x)}{dx} \right]$$

Recalling that  $f(x) = dF(x)/dx$  and that the derivative of a constant is 0, it follows that

$$-\frac{1}{1 - F(x)} \left[ \frac{d1}{dx} - \frac{dF(x)}{dx} \right] = -\frac{1}{1 - F(x)} [0 - f(x)]$$

Simplifying the expression by canceling out the minus signs and removing the 0, we get

$$-\frac{1}{1 - F(x)} [0 - f(x)] = \frac{f(x)}{1 - F(x)} = \frac{f(x)}{S(x)}$$

As we saw in Section 2.2,  $\frac{f(x)}{S(x)} = h(x)$ . Thus it follows that  $h(x) = -\frac{d \ln [S(x)]}{dx}$ . Q.E.D.

## 2.4 $H(x) = -\ln S(x)$

Since  $H(x) = \int_{-0}^x h(t)dt$ , it follows that

$$H(x) = -\ln S(x) \Leftrightarrow \int_{-0}^x h(t)dt = -\ln S(x)$$

Since  $\frac{dH(x)}{dx} = h(x)$ , it follows that

$$H(x) = -\ln S(x) \Leftrightarrow \frac{dH(x)}{dx} = -\frac{d \ln S(x)}{dx}$$

Thus it follows that  $H(x) = -\ln S(x)$  is true if  $\frac{dH(x)}{dx} = -\frac{d \ln S(x)}{dx}$  is true, which was proven in Section 2.3.

Q.E.D.